Updates.

FOL/Binders.lean
@@ -153,11 +153,30 @@ instance (v : VarName) (F : Formula) : Decidable (isFreeIn v F) :=
 
 
 /--
+  Formula.predVarSet F := The set of all of the predicate variables that have an occurrence in the formula F.
+-/
+def Formula.predVarSet : Formula → Finset (PredName × ℕ) 
+  | pred_const_ _ _ => ∅
+  | pred_var_ X xs => {(X, xs.length)}
+  | eq_ _ _ => ∅ 
+  | true_ => ∅
+  | false_ => ∅
+  | not_ phi => phi.predVarSet
+  | imp_ phi psi => phi.predVarSet ∪ psi.predVarSet
+  | and_ phi psi => phi.predVarSet ∪ psi.predVarSet
+  | or_ phi psi => phi.predVarSet ∪ psi.predVarSet
+  | iff_ phi psi => phi.predVarSet ∪ psi.predVarSet
+  | forall_ _ phi => phi.predVarSet
+  | exists_ _ phi => phi.predVarSet
+  | def_ _ _ => ∅
+
+
+/--
   predVarOccursIn P n F := True if and only if there is an occurrence of the predicate variable named P of arity n in the formula F.
 -/
 def predVarOccursIn (P : PredName) (n : ℕ) : Formula → Prop
   | pred_const_ _ _ => False
-  | pred_var_ X xs => X = P ∧ xs.length = n
+  | pred_var_ X xs => P = X ∧ n = xs.length
   | eq_ _ _ => False
   | true_ => False
   | false_ => False
@@ -301,6 +320,50 @@ theorem isFreeIn_iff_mem_freeVarSet
   case def_ X xs =>
     unfold isFreeIn
     unfold Formula.freeVarSet
+    simp
+
+
+theorem predVarOccursIn_iff_mem_predVarSet
+  (P : PredName)
+  (n : ℕ) 
+  (F : Formula) :
+  predVarOccursIn P n F ↔ (P, n) ∈ F.predVarSet :=
+  by
+  induction F
+  case pred_const_ X xs =>
+    unfold predVarOccursIn
+    unfold Formula.predVarSet
+    simp
+  case pred_var_ X xs =>
+    unfold predVarOccursIn
+    unfold Formula.predVarSet
+    simp
+  case eq_ x y =>
+    unfold predVarOccursIn
+    unfold Formula.predVarSet
+    simp
+  case true_ | false_ =>
+    unfold predVarOccursIn
+    unfold Formula.predVarSet
+    simp
+  case not_ _ phi_ih =>
+    exact phi_ih
+  case
+      imp_ phi psi phi_ih psi_ih
+    | and_ phi psi phi_ih psi_ih
+    | or_ phi psi phi_ih psi_ih
+    | iff_ phi psi phi_ih psi_ih =>
+    unfold predVarOccursIn
+    unfold Formula.predVarSet
+    simp
+    simp only [phi_ih, psi_ih]
+  case forall_ x phi phi_ih | exists_ x phi phi_ih =>
+    unfold predVarOccursIn
+    unfold Formula.predVarSet
+    exact phi_ih
+  case def_ X xs =>
+    unfold predVarOccursIn
+    unfold Formula.predVarSet
     simp
 
 
